cleanup

backends/lean/Aeneas/Tactic/Step/Tests/TupleDestruct.lean
@@ -1,3 +1,4 @@
+import Aeneas.Do
 import Aeneas.Std.Slice
 import Aeneas.Tactic.Step
 
@@ -18,5 +19,40 @@ theorem getPairAndUse_step (x : U32) (h : x.val + 2 ≤ U32.max) :
     getPairAndUse x ⦃ r => r.val = x.val + 2 ⦄ := by
   unfold getPairAndUse
   step*
+
+def twoNats : Result (Nat × Nat) :=
+  ok (1, 2)
+
+@[step]
+theorem twoNats_spec : twoNats ⦃ a b => a = 1 ∧ b = 2⦄ := by unfold twoNats; step*
+
+def fourNats : Result ((Nat × Nat) × (Nat × Nat)) :=
+  ok ((3, 4), (5, 6))
+
+@[step]
+theorem fourNats_spec : fourNats ⦃ (a, b) (c,d) => a = 3 ∧ b = 4 ∧ c = 5 ∧ d = 6⦄ := by
+  unfold fourNats; step*
+
+def testTuples : Result Nat := do
+  let (a, b) ← twoNats
+  let (c, d) ← twoNats
+  let ((a, b), (c, d)) ← fourNats
+  let ((e, f), (g, h)) ← fourNats
+  ok (a + f + g + d)
+
+/--
+info: Try this:
+
+  [apply]     simp only [step_simps]
+    let* ⟨ a, b, a_post1, a_post2 ⟩ ← twoNats_spec
+    let* ⟨ c, d, c_post1, c_post2 ⟩ ← twoNats_spec
+    let* ⟨ _, _, _ ⟩ ← fourNats_spec
+    let* ⟨ _, _, _ ⟩ ← fourNats_spec
+    agrind
+-/
+#guard_msgs in 
+example : testTuples ⦃ res => res = 18⦄ := by
+  unfold testTuples
+  step*?
 
 end step_tuple_destruct
